# Simplifying Boolean Expressions

## De-Morgan's Laws

#### First Law

$\neg(A \vee B) = \neg A \wedge \neg B$

#### Second Law

$\neg(A \wedge B) = \neg A \vee \neg B$

## General Rules

$X \wedge 0 = 0$

$X \wedge 1 = X$

$X \wedge X = X$

$X \wedge \neg X = 0$

$X \vee 0 = X$

$X \vee 1 = 1$

$X \vee X = X$

$X \vee \neg X = 1$

## Commutative Rules

$X \wedge Y = Y \wedge X$

$X \vee Y = Y \vee X$

## Associative Rules

$X \wedge (Y \wedge Z) = (X \wedge Y) \wedge Z$

$X \vee (Y \vee Z) = (X \vee Y) \vee Z$

## Distributive Rules

$X \wedge (Y \vee Z) = (X \wedge Y) \vee (X \wedge Z)$

$(X \vee Y) \wedge (W \vee Z) = (X \wedge W) \vee (X \wedge Z) \vee (Y \wedge W)
\vee (Y \wedge Z)$

## Absorption Rules

$X \vee (X \wedge Y) = X$

$X \wedge (X \vee Y) = X$

## Double Negation

$X = \neg \neg X$

